{
 "cells": [
  {
   "cell_type": "markdown",
   "id": "41940b8d",
   "metadata": {},
   "source": [
    "$\\textbf{Discrete Structures II - LECTURE 1 Assignments}$\n",
    "\n",
    "$\\textbf{Name:}$ Jyreneah Angel\n",
    "\n",
    "$\\textbf{Program and Year:}$ BSCS - 1\n",
    "\n",
    "$\\textbf{Class Schedule:}$ CIS 1203 - Group 3 (MW - 1:30-3:00 PM)"
   ]
  },
  {
   "cell_type": "markdown",
   "id": "188d623d-79cb-4d7e-aaed-112bb84d8d33",
   "metadata": {},
   "source": [
    "$\\textbf{Assignment}$\n",
    "Instructions:\n",
    "- Use latex.\n",
    "- Write your latex in jupyter notebook.\n",
    "- Push your answer to your github account.\n",
    "- Deadline is 2 weeks before finals.\n",
    "- Fail to submit 2 weeks before finals is an automatic 5.0 for this assignment.\n",
    "- Each problem is 25 points.\n",
    "\n",
    "****\n",
    "1. Recall the definition of a rational number, denoted as $\\mathbb{Q}$. Prove that the Euler's number $e = \\Sigma_{k=0}^\\infty \\frac{1}{k!} \\notin \\mathbb{Q}$. A factorial is defined as $k! = (k)(k-1)(k-2)(k-3)..., \\forall k \\in \\mathbb{Z}^+$, note that $0! = 1$. Furthermore, a sum notation $\\Sigma_{k=0}^\\infty k = 0+ 1 + 2 + 3 +....+...$\n",
    "\n",
    "**PROOF:**\n",
    "\n",
    "Using the proof of contradiction, we can prove that Euler's number $ e $ is not rational.\n",
    "\n",
    "Step 1: Let us assume that euler's number is a rational number.\n",
    "\n",
    "$$e \\in \\mathbb{Q}$$\n",
    "\n",
    "Step 2: Then, recall the definition of a rational number, represented as $\\mathbb{Q}$\n",
    "\n",
    "$$\n",
    "\\frac{a}{b} = \\mathbb{Q}\n",
    "$$\n",
    "\n",
    "Step 3: Suppose that the summation from k = 0 to $\\infty$ can be expressed in a simpler form\n",
    "\n",
    "$$\n",
    "    e = \\sum_{k=0}^\\infty \\frac{1}{k!} = \\frac{1}{0!} + \\frac{1}{1!} + \\frac{1}{2!} ... + \\frac{1}{k!} = \\frac{a}{b}\n",
    "$$\n",
    "\n",
    "$$\n",
    "e = \\frac{a}{b}\n",
    "$$\n",
    "\n",
    "According to our hypothesis where $e \\in \\mathbb{Q}$, the reciprocal of eulers number\n",
    "should also be rational\n",
    "\n",
    "$$\n",
    "e = \\frac{a}{b} \\quad = \\quad e^{x} = \\frac{b}{a}\n",
    "$$\n",
    "$$\n",
    "s.t. \\space\\space x = -1\n",
    "$$\n",
    "\n",
    "$$\n",
    "e^{-1} = \\frac{1}{e} = \\frac{b}{a} = \\sum_{k=0}^\\infty \\frac{(-1)^{k}}{k!}\n",
    "$$\n",
    "\n",
    "$$\n",
    "s.t. \\space\\space\\space a,b \\in \\mathbb{Z}\n",
    "$$\n",
    "\n",
    "Step 4: Let's use 𝑎 to split the summation of the infinite series into two parts. The first part will be the summation from 0 to \n",
    "𝑎, and the second part will be the summation from 𝑎 to infinity.\n",
    "\n",
    "$$\n",
    "e^{-1} = \\frac{b}{a}= \\sum_{k=0}^{a} \\frac{(-1)^{k}}{k!} + \\sum_{k = a + 1}^{\\infty} \\frac{(-1)^{k}}{k!}\n",
    "$$\n",
    "\n",
    "$$\n",
    "\\frac{b}{a} - \\sum_{k = 0}^{a} \\frac{(-1)^k}{k!} = \\sum_{k = a + 1}^{\\infty} \\frac{(-1)^{k}}{k!}\n",
    "$$\n",
    "\n",
    "Step 5: After, multiply the terms with \n",
    "\n",
    "$$(-1)^{(a+1)}a!$$\n",
    "\n",
    "$\\textbf{term 1:}$\n",
    "\n",
    "$$\n",
    "= \\frac{b}{a} * (-1)^{(a+1)}a!\n",
    "$$\n",
    "\n",
    "$$\n",
    "    = (-1)^{(a+1)} b(a-1)! \n",
    "$$\n",
    "\n",
    "$\\textbf{term 2:}$\n",
    "\n",
    "$$\n",
    "(-1)^{(a+1)} (\\frac{a!}{2!} \\dots + \\frac{(-1)^{a}a!}{a})\n",
    "$$\n",
    "\n",
    "Since every denominator is always less than the numerator and is a factor of the numerator, the result will always be an integer\n",
    "\n",
    "$$\n",
    "    \\forall a, b \\in \\mathbb{Z}, a > b\n",
    "$$\n",
    "\n",
    "$$\n",
    "    \\frac{a!}{b!} = c, \\space\\space\\space s.t \\space\\space\\space c \\in \\mathbb{Z}\n",
    "$$\n",
    "\n",
    "As you can see, term 1 and term 2 is a subtraction between two integers, we can conclude that the left\n",
    "side of the equation is an integer\n",
    "\n",
    "$$\n",
    "(-1)^{(a+1)} b(a-1)! - (-1)^{(a+1)} (\\frac{a!}{2!} \\dots + \\frac{(-1)^{a}a!}{a}) \\in \\mathbb{Z}\n",
    "$$\n",
    "\n",
    "Let us expound on the term on the right side of the equation\n",
    "\n",
    "$$\n",
    "=  \\frac{1}{a + 1} - \\frac{1}{(a + 1)(a + 2)} + \\dots\n",
    "$$\n",
    "\n",
    "An upper and lower bound is definedin this expression. The first term is the \n",
    "upper bound. The succeeding terms are the lower bound such that it is lower than the first term\n",
    "as k reaches infinity, the summation of the succeding terms will approach zero. Therefore this\n",
    "this expression will result in a number that is irrational\n",
    "\n",
    "$$\n",
    "\\frac{1}{a + 1} - \\frac{1}{(a + 1)(a + 2)} + \\dots \\notin \\mathbb{Z}\n",
    "$$\n",
    "\n",
    "Since assuming $ e $ to a rational leads to a contradiction, it is concluded that Euler's number $ e $ is irrational."
   ]
  },
  {
   "cell_type": "markdown",
   "id": "6498d691",
   "metadata": {},
   "source": [
    "****\n",
    "2. Prove Minkowski's Inequality for sums, $\\forall \\ p>1, (a_k, b_k)>0$:\n",
    "\n",
    "\\begin{gather}\n",
    "\\begin{bmatrix}\n",
    "\\Sigma_{k=1}^n |a_k + b_k|^p\n",
    "\\end{bmatrix}^\\frac{1}{p}\n",
    "\\leq\n",
    "\\begin{bmatrix}\n",
    "\\Sigma_{k=1}^n |a_k|^p\n",
    "\\end{bmatrix}^\\frac{1}{p}\n",
    "\n",
    "\\begin{bmatrix}\n",
    "\\Sigma_{k=1}^n |b_k|^p\n",
    "\\end{bmatrix}^\\frac{1}{p}\n",
    "\\end{gather}\n",
    "\n",
    "**PROOF:**\n",
    "\n",
    "Let us directly prove Minskowski's Inequality for sums by the\n",
    "triangle Inequality theorem\n",
    "\n",
    "$$\n",
    "|a + b| \\leq |a| + |b|\n",
    "$$\n",
    "\n",
    "Step 1: Let us raise terms on both sides to P\n",
    "\n",
    "$$\n",
    "|a + b|^{p} \\leq |a|^{p} + |b|^{p}  \n",
    "$$\n",
    "\n",
    "Step 2: Do summation notation for all k from 1 to n\n",
    "\n",
    "$$\n",
    "\\sum_{k = 1}^{n} |a_k + b_k|^{p} \\leq \\sum_{k=1}^{n} |a_k|^{p} + \\sum_{k =1 }^{n} |b_k|^{p} \n",
    "$$\n",
    "\n",
    "Step 3: Raise to 1 over p by property of absolute value\n",
    "\n",
    "$$\n",
    "[\\sum_{k = 1}^{n}|a_k + b_k|^{p}]^{\\frac{1}{p}} \\leq [\\sum_{k = 1}^{n} |a_k|^{p}]^{\\frac{1}{p}} + [\\sum_{k = 1}^{n}|b_k|^{p}]^{\\frac{1}{p}}\n",
    "$$\n",
    "\n",
    "Thus, Minkowski's Inequality for sums is proven by using the Triangle Inequality theorem. \n"
   ]
  },
  {
   "cell_type": "markdown",
   "id": "d1f25513",
   "metadata": {},
   "source": [
    "****\n",
    "3. Prove the triangle inequality $|x+y| \\leq |x| + |y|, \\forall (x,y) \\in \\mathbb{R}$\n",
    "\n",
    "**PROOF:** \n",
    "\n",
    "Let us directly prove by referencing the square of a binomial\n",
    "\n",
    "Recall\n",
    "\n",
    "$$\n",
    "(x + y)^{2} = x^{2} + 2xy + y^{2}\n",
    "$$\n",
    "\n",
    "By known property of absolute value, we know that\n",
    "\n",
    "$$\n",
    "x \\leq |x|\\\\\n",
    "y \\leq |y|\\\\\n",
    "$$\n",
    "\n",
    "These inequalities are true for all Real Numbers\n",
    "\n",
    "$$\n",
    "x^{2} + 2xy + y^{2} \\leq |x|^{2} + 2|x||y| + |x|^{2}\n",
    "$$\n",
    "\n",
    "$$\n",
    "(x+y)^{2} \\leq |x|^{2} + 2|x||y| + |y|^{2}\n",
    "$$\n",
    "\n",
    "factor out $2|x||y|$\n",
    "\n",
    "$$\n",
    "(x+y)^{2} \\leq |x|^{2} + |y|^{2}\n",
    "$$\n",
    "\n",
    "By known property of absolute values, we know that\n",
    "\n",
    "$$\n",
    "\\forall x \\in \\mathbb{R}\\\\\n",
    "\n",
    "\\sqrt{x^{2}} = |x|\\\\\n",
    "$$\n",
    "\n",
    "Therefore if we square root all terms,\n",
    "\n",
    "$$\n",
    "\\sqrt{(x+y)^{2}} \\leq \\sqrt{|x|^{2}} + \\sqrt{|y|^{2}}\n",
    "$$\n",
    "\n",
    "Is equivalent to\n",
    "\n",
    "$$\n",
    "|x + y| \\leq |x| + |y|\n",
    "$$\n",
    "\n",
    "Thus, the proof establishes the triangle inequality by directly referencing the square of a binomial. "
   ]
  },
  {
   "cell_type": "markdown",
   "id": "284d120f",
   "metadata": {},
   "source": [
    "****\n",
    "4. Prove Sedrakayan's Lemma $\\forall u_i, v_i \\in \\mathbb{R}^+$:\n",
    "\\begin{gather}\n",
    "\\frac{(\\Sigma_{i=1}^n u_i)^2}{\\Sigma_{i=1}^n v_i}\n",
    "\\leq\n",
    "\\Sigma_{i=1}^n \\frac{(u_i)^2}{v_i}\n",
    "\\end{gather}\n",
    "\n",
    "**PROOF:**\n",
    "\n",
    "Recall the Cauchy-Schwarz Inequality:\n",
    "\n",
    "$$\n",
    "|<a,b>|^{2} \\leq\\space\\space <a,a><b,b>\n",
    "$$\n",
    "\n",
    "$$\n",
    "\\forall u_i, v_i \\in \\mathbb{R}^{+}\n",
    "$$\n",
    "\n",
    "Let $a_i = u_i, b_i = \\sqrt{v_i}$\n",
    "\n",
    "$$\n",
    "|<a,b>|^{2}=(\\sum_{i = 1}^{n}a_ib_i)^{2} = (\\sum_{i = 1}^{n}u_i \\sqrt{v_i})^{2}\\\\\n",
    "$$\n",
    "$$\n",
    "<a,a><b,b>=(\\sum_{i = 1}^{n}a_i^{2})(\\sum_{i = 1}^{n}b_i^{2}) = (\\sum_{i = 1}^{n} u_i^{2})(\\sum_{i = 1}^{n}v_i)\\\\\n",
    "$$\n",
    "\n",
    "Thus,\n",
    "\n",
    "$$\n",
    "(\\sum_{i = 1}^{n}u_i \\sqrt{v_i})^{2} \\leq (\\sum_{i = 1}^{n} u_i^{2})(\\sum_{i = 1}^{n}v_i)\n",
    "$$\n",
    "\n",
    "Dividing both sides by $\\sum_{i=1}^{n}v_i$, we obtain:\n",
    "\n",
    "$$\n",
    "\\frac{(\\sum_{i=1}^{n}u_i)^{2}}{\\sum_{i=1}^{n}v_i} \\leq \\sum_{i = 1}^{n} \\frac{u_i^{2}}{v_i}\n",
    "$$\n",
    "\n",
    "Hence, Sedrakayan's Lemma is proven."
   ]
  },
  {
   "cell_type": "markdown",
   "id": "1de33a92-7a6a-4624-a8c5-994644cffc20",
   "metadata": {},
   "source": [
    "****\n",
    "1. Consider the functions $f(x) = 2x+1$, $g(x)=2y-1$, $j(x) = |f(x)+g(x)|$, and $h(x) = j(x)^2$, show for the following inequality that:\n",
    "\n",
    "\\begin{gather}\n",
    "\\sqrt{|f(x)|^2} \\geq \\sqrt{h(x)} - \\sqrt{|g(x)|^2}, \\forall (x,y) \\in \\mathbb{Z}^+\n",
    "\\end{gather}\n",
    "\n",
    "**PROOF:**\n",
    "\n",
    "To prove the inequality, start by substituting the given functions:\n",
    "\n",
    "$$\n",
    "\\sqrt{(2x+1)^{2}} \\geq \\sqrt{|(2x + 1)+(2y - 1)|^{2}} - \\sqrt{(2y-1)^{2}}\n",
    "$$\n",
    "\n",
    "By properties of absolute value, we know that\n",
    "\n",
    "$$\n",
    "\\sqrt{(x)^{2}} = |x|\n",
    "$$\n",
    "\n",
    "Therefore, we get\n",
    "\n",
    "$$\n",
    "|2x + 1| \\geq |(2x + 1) + (2y - 1)| - |2y - 1|\n",
    "$$\n",
    "\n",
    "Let us assign variables to simplify the expression, such that $a = 2x + 1$ and $b = 2y - 1$. Then we rewrite the inequality as:\n",
    "\n",
    "$$\n",
    "|a| \\geq |a + b| - |b|\n",
    "$$\n",
    "\n",
    "By adding |b| and subtracting |a| to both sides and we get:\n",
    "\n",
    "$$\n",
    "|a + b| \\leq |a| + |b|\n",
    "$$\n",
    "\n",
    "This inequality is known as the triangle inequality theorem.\n",
    "\n",
    "Thus, the given inequality follows from the triangle inequality theorem."
   ]
  },
  {
   "cell_type": "markdown",
   "id": "997eb723-4112-443b-92d6-4f6734ea8e3b",
   "metadata": {},
   "source": [
    "****\n",
    "2. Prove Sedrakayan's Lemma if $u_i, v_i$ are square roots of an even integers:\n",
    "\\begin{gather}\n",
    "\\frac{(\\Sigma_{i=1}^n u_i)^2}{\\Sigma_{i=1}^n v_i}\n",
    "\\leq\n",
    "\\Sigma_{i=1}^n \\frac{(u_i)^2}{v_i}\n",
    "\\end{gather}\n",
    "\n",
    "**PROOF:**\n",
    "\n",
    "recalling the Cauchy-Schwarz inequality for Real Numbers...\n",
    "\n",
    "$$\n",
    "(\\sum_{i=1}^{n}a_i b_i)^{2} \\leq (\\sum_{i=1}^{n}a_i^{2})(\\sum_{i=1}^{n}b_i^{2})\n",
    "$$\n",
    "\n",
    "let $a_i = u_i$ and $b_i = \\sqrt{v_i}$\n",
    "\n",
    "$$\n",
    "(\\sum_{i=1}^{n}u_i \\sqrt{v_i})^{2} \\leq (\\sum_{i=1}^{n}u_i^{2})(\\sum_{i=1}^{n}\\sqrt{v_i}^{2})\n",
    "$$\n",
    "\n",
    "since we are dealing with the square root of even integers, substitute the values $u_i = \\sqrt{2a_i}, \\sqrt{v_i} = \\sqrt{2b_i}$\n",
    "\n",
    "$$\n",
    "(\\sum_{i=1}^{n}\\sqrt{2a_i}\\sqrt{2b_i})^{2} \\leq (\\sum_{i=1}^{n}[\\sqrt{2a_i}]^{2})(\\sum_{i=1}^{n}[\\sqrt{2b_i}]^{2})\n",
    "$$\n",
    "\n",
    "simplify\n",
    "\n",
    "$$\n",
    "4\\sum_{i=1}^{n}a_ib_i \\leq 4\\sum_{i=1}^{n}a_i\\sum_{i=1}^{n}b_i\n",
    "$$\n",
    "\n",
    "divide both sides by... $4\\sum_{i=1}^{n}b_i$\n",
    "\n",
    "$$\n",
    "\\frac{4\\sum_{i=1}^{n}a_ib_i \\leq 4\\sum_{i=1}^{n}a_i\\sum_{i=1}^{n}b_i}{4\\sum_{i=1}^{n}b_i}\n",
    "$$\n",
    "\n",
    "$$\n",
    "4(\\frac{1}{4} )\\space [\\sum_{i=1}^{n}a_ib_i (\\frac{1}{[\\sum_{i=1}^{n}b_i]})] \\leq 4(\\frac{1}{4})\\space \\sum_{i=1}^{n}a_i(\\frac{1}{[\\sum_{i=1}^{n}b_i]})\\space\\space \\sum_{i=1}^{n}b_i (\\frac{1}{[\\sum_{i=1}^{n}b_i]})\n",
    "$$\n",
    "\n",
    "$$\n",
    "\\frac{\\sum_{i=1}^{n}a_i}{\\sum_{i=1}^{n}b_i} \\leq \\sum_{i=1}^{n}\\frac{a_i}{b_i}\n",
    "$$\n",
    "\n",
    "Remember that $u_i = \\sqrt{2a_i}, v_i = \\sqrt{2b_i}$\n",
    "\n",
    "modify the equality to get $a$ and $b$\n",
    "\n",
    "$$\n",
    "u_i = \\sqrt{2a_i}\n",
    "$$\n",
    "$$\n",
    "a = (\\frac{u_i^{2}}{2})\n",
    "$$\n",
    "\n",
    "$$\n",
    "\\sqrt{v_i} = \\sqrt{2b_i}\n",
    "$$\n",
    "$$\n",
    "b = (\\frac{\\sqrt{v_i}^{2}}{2})\n",
    "$$\n",
    "\n",
    "Substitue and square the numerator to get Sedrakayan's Lemma\n",
    "\n",
    "$$\n",
    "\\frac{\\sum_{i=1}^{n}\\frac{u_i^{2}}{2}}{\\sum_{i=1}^{n}\\frac{\\sqrt{v_i}^{2}}{2}} \\leq \\sum_{i=1}^{n}\\frac{\\frac{u_i^{2}}{2}}{\\frac{\\sqrt{v_i}^{2}}{2}}\n",
    "$$\n",
    "\n",
    "$$\n",
    "\\frac{(\\sum_{i=1}^{n}u_i)^{2}}{\\sum_{i=1}^{n}v_i} \\leq \\sum_{i=1}^{n}\\frac{u_i^{2}}{v_i}\n",
    "$$\n",
    "\n",
    "Therefore, Sedrakyan's Lemma holds true for $ u_i $ and $ v_i $ being square roots of even integers."
   ]
  }
 ],
 "metadata": {
  "kernelspec": {
   "display_name": "Python 3 (ipykernel)",
   "language": "python",
   "name": "python3"
  },
  "language_info": {
   "codemirror_mode": {
    "name": "ipython",
    "version": 3
   },
   "file_extension": ".py",
   "mimetype": "text/x-python",
   "name": "python",
   "nbconvert_exporter": "python",
   "pygments_lexer": "ipython3",
   "version": "3.8.16"
  }
 },
 "nbformat": 4,
 "nbformat_minor": 5
}
